templates/multicopy/multicopy_client_level.v
@@ -19,9 +19,9 @@ Definition search' : val :=
   λ: "k",
     let: "t_id" := NewProph in
     let: "p" := NewProph in
-    let: "vt'" := search "k" in
-    resolve_proph: "p" to: "vt'";;
-    "vt'".  
+    let: "v" := search "k" in
+    resolve_proph: "p" to: "v";;
+    "v".  
 
 Section multicopy_client_level.
   Context {Σ} `{heapG Σ, !multicopyG Σ}.
@@ -32,10 +32,10 @@ Section multicopy_client_level.
   Parameter search_recency: ∀ N γ_te γ_he γ_s Prot Inv_tpl k v0 t0, 
     ⊢ ⌜k ∈ KS⌝ -∗ 
         mcs_inv N γ_te γ_he γ_s Prot Inv_tpl -∗
-          SR γ_s (k, v0, t0) -∗
+          SR γ_s (k, (v0, t0)) -∗
               <<< True >>> 
                   search #k @ ⊤ ∖ ↑(mcsN N)
-              <<< ∃ (v: V) (t: TS), SR γ_s (k, v, t) ∗ ⌜t0 ≤ t⌝ , RET (#v, #t) >>>.
+              <<< ∃ (v: V) (t: T), SR γ_s (k, (v, t)) ∗ ⌜t0 ≤ t⌝ , RET #v >>>.
 
   Parameter upsert_spec: ∀ N γ_te γ_he γ_s Prot Inv_tpl k (v: V),
     ⊢ ⌜k ∈ KS⌝ -∗ 
@@ -43,7 +43,7 @@ Section multicopy_client_level.
           mcs_inv N γ_te γ_he γ_s Prot Inv_tpl -∗
               <<< ∀ t H, MCS γ_te γ_he t H >>> 
                      upsert #k #v @ ⊤ ∖ (↑(mcsN N))
-              <<< MCS γ_te γ_he (t + 1) (H ∪ {[(k, v, t)]}), RET #() >>>.
+              <<< MCS γ_te γ_he (t + 1) (H ∪ {[(k, (v, t))]}), RET #() >>>.
                 
   (** Proof of high-level specs for multicopy opeartions *)                
 
@@ -52,104 +52,69 @@ Section multicopy_client_level.
       mcs_inv N γ_te γ_he γ_s (Prot_help N γ_te γ_he γ_td γ_ght) Inv_tpl -∗ 
           <<< ∀ t H, MCS γ_te γ_he t H >>>
                 search' #k @ ⊤ ∖ (↑(mcsN N) ∪ ↑(threadN N))
-          <<<  ∃ (vt: V * TS), MCS γ_te γ_he t H 
-                            ∗ ⌜map_of_set H !!! k = vt⌝, RET (#vt.1, #vt.2) >>>.
+          <<<  ∃ (v': V) (t': T), MCS γ_te γ_he t H 
+                            ∗ ⌜map_of_set H !!! k = (v', t')⌝, RET #v' >>>.
   Proof.
     iIntros "% #HInv" (Φ) "AU". wp_lam.
     rename H0 into k_in_KS.
     wp_apply wp_new_proph1; try done.
-    iIntros (tid vt)"Htid". wp_pures.
-    wp_apply (typed_proph_wp_new_proph1 VTTypedProph); first done.
-    iIntros (vtp p)"Hproph". wp_pures. 
+    iIntros (tid vtid)"Htid". wp_pures.
+    wp_apply (typed_proph_wp_new_proph1 IntTypedProph); first done.
+    iIntros (vp p)"Hproph". wp_pures. 
     iApply fupd_wp.
     iInv "HInv" as (T0 H0) "(mcs_high & Htpl)".
-    iDestruct "mcs_high" as "(>MCS_auth & >HH & >Hist & >MaxTS & >Uniq & Prot)".
-    iAssert (⌜∃ v0 t0, ((k, v0, t0) ∈ H0 ∧ (∀ v t, (k, v, t) ∈ H0 → t ≤ t0) 
+    iDestruct "mcs_high" as "(>MCS_auth & >HH & >HInit & >HClock & >HUniq & Prot)".
+    iAssert (⌜∃ v0 t0, ((k, (v0, t0)) ∈ H0 ∧ (∀ v t, (k, (v, t)) ∈ H0 → t ≤ t0) 
                 ∧ map_of_set H0 !! k = Some (v0, t0))⌝)%I as "%".
     { pose proof (map_of_set_lookup_cases H0 k) as H'.
       destruct H' as [H' | H']; try done.
-      iDestruct "Hist" as %Hist.
+      iDestruct "HInit" as %HInit.
       destruct H' as [H' _].
-      pose proof H' 0%Z 0 as H'.
-      pose proof Hist k k_in_KS as Hist.
+      pose proof H' bot 0 as H'.
+      pose proof HInit k k_in_KS as HInit.
       contradiction. }
 
     destruct H1 as [v0 [t0 [kt0_in_H [Max_t0 H_k]]]].
-    iMod (own_update γ_s (● H0) (● H0 ⋅ ◯ {[(k, v0, t0)]}) with "[$HH]") as "HH".
-    { apply (auth_update_frac_alloc _ H0 ({[(k, v0, t0)]})).
+    iMod (own_update γ_s (● H0) (● H0 ⋅ ◯ {[(k, (v0, t0))]}) with "[$HH]") as "HH".
+    { apply (auth_update_frac_alloc _ H0 ({[(k, (v0, t0))]})).
       apply gset_included. clear -kt0_in_H. set_solver. }
-    iDestruct "HH" as "(HH & #mcs_sr)".
+    iDestruct "HH" as "(HH & #SR0)".
                      
-    destruct (decide (vtp.2 ≤ t0)).
-    - assert ((vtp.2 < t0) ∨ vtp.2 = t0) as H' by lia.
-      destruct H' as [Hcase' | Hcase'].
-      + iModIntro. iSplitR "AU Hproph".
-        iNext; iExists T0, H0; iFrame.
-        iModIntro.
-        awp_apply search_recency; try done.
-        iAaccIntro with ""; try done.
-        { iIntros "_". iModIntro; try eauto with iFrame. } 
-        iIntros (v t) "(Hkt & %)". rename H1 into t0_le_t.
-        iModIntro. wp_pures.
-        wp_apply (typed_proph_wp_resolve1 VTTypedProph with "Hproph"); try done.
-        wp_pures. iModIntro. iIntros "%". rename H1 into tp_eq_t.
-        clear -tp_eq_t Hcase' t0_le_t. rewrite tp_eq_t in Hcase'.
-        simpl in Hcase'. exfalso; lia.
-      + iMod "AU" as (T' H') "[MCS [_ Hcomm]]".
-        set_solver.
-        iAssert (⌜T' = T0 ∧ H' = H0⌝)%I as "%". 
-        { iPoseProof (MCS_agree with "[$MCS_auth] [$MCS]") as "(% & %)".
-          by iPureIntro. }
-        destruct H1 as [H'' H''']. subst T' H'.
-        assert (map_of_set H0 !!! k = (v0, t0)) as M_k.
-        { rewrite lookup_total_alt. rewrite H_k.
-          by simpl. }
-        iSpecialize ("Hcomm" $! (v0, t0)). 
-        iMod ("Hcomm" with "[MCS]") as "HΦ".
-        { iFrame. by iPureIntro. } 
-        iModIntro. iSplitR "HΦ Hproph".
-        iNext; iExists T0, H0; iFrame.
-        iModIntro.
-        awp_apply search_recency without "HΦ"; try done.
-        iAaccIntro with ""; try done.
-        { iIntros "_". iModIntro; try eauto with iFrame. } 
-        iIntros (v t) "(#Hkt & %)". rename H1 into t0_le_t.
-        iModIntro. iIntros "HΦ". wp_pures.
-        wp_apply (typed_proph_wp_resolve1 VTTypedProph with "Hproph"); try done.
-        wp_pures. iModIntro. iIntros "%". rename H1 into tp_eq_t. 
-        wp_pures.
-        iInv "HInv" as (T1 H1) "(mcs_high & Htpl)".
-        iDestruct "mcs_high" as "(>MCS_auth & >HH & >Hist & >MaxTS & >Uniq & Prot)".
-        iDestruct "Uniq" as %Uniq.
-        iPoseProof (auth_own_incl γ_s H1 _ with "[$HH $mcs_sr]") as "%".
-        rename H2 into vt0_sub_H1.
-        apply gset_included in vt0_sub_H1.
-        assert ((k,v0,t0) ∈ H1) as vt0_in_H1 by set_solver.
-        iPoseProof (auth_own_incl γ_s H1 _ with "[$HH $Hkt]") as "%".
-        rename H2 into vt_sub_H1.
-        apply gset_included in vt_sub_H1.
-        assert ((k,v,t) ∈ H1) as vt_in_H1 by set_solver.
-        iModIntro. iSplitR "HΦ".
-        iNext; iExists T1, H1; iFrame"∗%". iModIntro.
-        
-        assert (vtp.2 = t) as H'.
-        { rewrite tp_eq_t. simpl. by lia. }
-        rewrite <-H'. rewrite Hcase'.
-        rewrite <-H' in vt_in_H1; rewrite Hcase' in vt_in_H1.
-        pose proof Uniq k v0 v t0 vt0_in_H1 vt_in_H1 as Uniq.
-        by rewrite Uniq.
-    - assert (vtp.2 > t0) by lia. rename H1 into tp_gr_t0.
-      iDestruct "Prot" as (R hγt)"(>HR & >Hγt 
+    destruct (decide (v0 = vp)) as [v0_eq_vp | v0_neq_vp].
+    - iMod "AU" as (T' H') "[MCS [_ Hcomm]]"; first by set_solver.
+      iAssert (⌜T' = T0 ∧ H' = H0⌝)%I as "%". 
+      { iPoseProof (MCS_agree with "[$MCS_auth] [$MCS]") as "(% & %)".
+        by iPureIntro. }
+      destruct H1 as [H'' H''']. subst T' H'.
+      assert (map_of_set H0 !!! k = (v0, t0)) as M_k.
+      { rewrite lookup_total_alt. rewrite H_k.
+        by simpl. }
+      iSpecialize ("Hcomm" $! v0 t0). 
+      iMod ("Hcomm" with "[MCS]") as "HΦ".
+      { iFrame. by iPureIntro. } 
+      iModIntro. iSplitR "HΦ Hproph".
+      iNext; iExists T0, H0; iFrame.
+      iModIntro.
+      awp_apply search_recency without "HΦ"; try done.
+      iAaccIntro with ""; try done.
+      { iIntros "_". iModIntro; try eauto with iFrame. } 
+      iIntros (v t) "(#SR & %)". rename H1 into t0_le_t.
+      iModIntro. iIntros "HΦ". wp_pures.
+      wp_apply (typed_proph_wp_resolve1 IntTypedProph with "Hproph"); try done.
+      wp_pures. iModIntro. iIntros "%". rename H1 into vp_eq_v. 
+      wp_pures. iModIntro.
+      by subst v vp.
+    - iDestruct "Prot" as (R hγt)"(>HR & >Hγt 
                                       & >Domm_hγt & Hstar_reg)".
       iAssert (▷ (⌜tid ∉ R⌝ 
                 ∗ ([∗ set] t_id ∈ R, Reg N γ_te γ_he γ_ght H0 t_id) 
-                ∗ proph1 tid vt))%I with "[Hstar_reg Htid]" 
+                ∗ proph1 tid vtid))%I with "[Hstar_reg Htid]" 
                 as "(>% & Hstar_reg & Htid)".
       { destruct (decide (tid ∈ R)); try done.
         - iEval (rewrite (big_sepS_elem_of_acc _ (R) tid); 
                                 last by eauto) in "Hstar_reg".
           iDestruct "Hstar_reg" as "(Hreg & Hstar_reg')".
-          iDestruct "Hreg" as (? ? ? ? ? ? ?)"(H' & _)".
+          iDestruct "Hreg" as (? ? ? ? ? ? ? ?)"(H' & _)".
           iAssert (▷ False)%I with "[H' Htid]" as "HF".
           iApply (proph1_exclusive tid with "[Htid]"); try done.
           iNext. iExFalso; try done.
@@ -184,12 +149,15 @@ Section multicopy_client_level.
                   
       iDestruct (laterable with "AU") as (AU_later) "[AU #AU_back]".
       iMod (own_alloc (Excl ())) as (γ_tk') "Token"; first try done.
-      assert (∀ v, (k, v, vtp.2) ∉ H0) as ktp_notin_H. 
-      { intros v. destruct (decide ((k, v, vtp.2) ∈ H0)); try done.
-        pose proof Max_t0 v vtp.2 e as H'.
-        clear -H' tp_gr_t0. lia. } 
+      iAssert (⌜(∀ t', (k, (vp, t')) ∈ H0 → t' < t0)⌝)%I as %HPending. 
+      { iDestruct "HUniq" as %HUniq. iPureIntro. 
+        intros t' kvpt'_in_H. pose proof Max_t0 vp t' kvpt'_in_H as Max_t0.
+        destruct (decide (t0 = t')).
+        - subst t'. pose proof HUniq k t0 v0 vp kt0_in_H kvpt'_in_H as HUniq.
+          done.
+        - clear - Max_t0 n. lia. }
       iMod (inv_alloc (threadN N) _
-              (∃ H, State γ_sy tid γ_tk' AU_later (Φ) H k vtp) 
+              (∃ H, State γ_sy tid γ_tk' AU_later (Φ) H k vp t0) 
                                     with "[AU Hreg_sy1]") as "#HthInv".
       { iNext. iExists H0. iFrame "Hreg_sy1". iLeft. 
         unfold Pending. iFrame. by iPureIntro. }
@@ -202,7 +170,7 @@ Section multicopy_client_level.
       rewrite Domm_hγt. clear; set_solver.
       rewrite (big_sepS_delete _ (R ∪ {[tid]}) tid); last by set_solver.
       iSplitR "Hstar_reg". unfold Reg.
-      iExists AU_later, Φ, k, vtp, vt, γ_tk', γ_sy. iFrame "∗#".
+      iExists AU_later, Φ, k, vp, t0, vtid, γ_tk', γ_sy. iFrame "∗#".
       assert ((R ∪ {[tid]}) ∖ {[tid]} = R) as H' 
                   by (clear -tid_notin_R; set_solver).
       by rewrite H'.
@@ -210,10 +178,10 @@ Section multicopy_client_level.
       iModIntro. awp_apply search_recency; try done.
       iAaccIntro with ""; try done.
       { iIntros "_". iModIntro; try eauto with iFrame. } 
-      iIntros (v t) "(#Hkt & %)". rename H1 into t0_le_t.
+      iIntros (v t) "(#SR & %)". rename H1 into t0_le_t.
       iModIntro. wp_pures.
-      wp_apply (typed_proph_wp_resolve1 VTTypedProph with "Hproph"); try done.
-      wp_pures. iModIntro. iIntros "%". rename H1 into tp_eq_t.
+      wp_apply (typed_proph_wp_resolve1 IntTypedProph with "Hproph"); try done.
+      wp_pures. iModIntro. iIntros "%". subst v. (* rename H1 into vp_eq_v. *)
       iApply fupd_wp.
       iInv "HthInv" as (H1)"(>Hth_sy & Hth_or)".
       iInv "HInv" as (T1 H1') "(mcs_high & Htpl)".
@@ -235,7 +203,7 @@ Section multicopy_client_level.
       { iEval (rewrite (big_sepS_elem_of_acc _ (R1) tid); 
                                 last by eauto) in "Hstar_reg".
         iDestruct "Hstar_reg" as "(Hreg_t & Hstar_reg')".
-        iDestruct "Hreg_t" as (P' Q' k' vp' vt' γ_tk'' γ_sy')
+        iDestruct "Hreg_t" as (P' Q' k' vp' t0' vtid' γ_tk'' γ_sy')
                           "(Hreg_proph & >Hreg_gh' & >Hreg_sy & Ht_reg')".
 
         iCombine "Hreg_gh" "Hreg_gh'" as "H".
@@ -255,20 +223,31 @@ Section multicopy_client_level.
           by iPureIntro. } subst H1'.
         iSplitR. iNext; by iPureIntro.
         iSplitR "Hth_sy". iApply "Hstar_reg'".
-        iNext. iExists P', Q', k', vp', vt', γ_tk'', γ_sy.
+        iNext. iExists P', Q', k', vp', t0', vtid', γ_tk'', γ_sy.
         iFrame "∗#". by iNext. } subst H1'.
-      assert (vtp.2 = t) as H' by (rewrite tp_eq_t; simpl; lia). 
-      iAssert (⌜(k, vtp.1, vtp.2) ∈ H1⌝)%I as "%". 
-      { iPoseProof (own_valid_2 _ _ _ with "[$HH] [$Hkt]") as "H'".
+      iAssert (⌜(k, (v0, t0)) ∈ H1⌝)%I as %kv0t0_in_H1.
+      { iPoseProof (own_valid_2 _ _ _ with "[$HH] [$SR0]") as "H'".
         iDestruct "H'" as %H''.
         apply auth_both_valid_discrete in H''.
         destruct H'' as [H'' _].
         apply gset_included in H''.
-        rewrite tp_eq_t; simpl.
-        rewrite tp_eq_t in H'; simpl in H'.
-        rewrite H'.
-        iPureIntro; clear -H''; set_solver. }
-      rename H0 into ktp_in_H1.
+        iPureIntro. clear -H''; by set_solver. }  
+      iAssert (⌜(k, (vp, t)) ∈ H1⌝)%I as %kvpt_in_H1.
+      { iPoseProof (own_valid_2 _ _ _ with "[$HH] [$SR]") as "H'".
+        iDestruct "H'" as %H''.
+        apply auth_both_valid_discrete in H''.
+        destruct H'' as [H'' _].
+        apply gset_included in H''.
+        iPureIntro. clear -H''; by set_solver. }  
+      iAssert (⌜¬ (∀ t' : nat, (k, (vp, t')) ∈ H1 → t' < t0)⌝)%I as "%". 
+      { iDestruct "Uniq" as %Uniq.
+        iPureIntro. intros H'.
+        pose proof H' t kvpt_in_H1 as H'.
+        destruct (decide (t = t0)).
+        - subst t. 
+          pose proof Uniq k t0 vp v0 kvpt_in_H1 kv0t0_in_H1 as Uniq.
+          apply v0_neq_vp. done.
+        - clear -t0_le_t n H'. lia. }  
       iDestruct "Hth_or" as "[Hth_or | Hth_or]".
       { iDestruct "Hth_or" as "(? & >%)".
         exfalso. try done. }
@@ -285,66 +264,81 @@ Section multicopy_client_level.
       iNext. iExists H1. iFrame "Hth_sy". 
       iRight. iFrame "∗%".
       
-      iModIntro. wp_pures. iModIntro.
-      iEval (rewrite tp_eq_t; simpl) in "Hth_or".
-      assert (Z.to_nat t = t) as Ht by lia.
-      by iEval (rewrite Ht) in "Hth_or".
+      iModIntro. wp_pures. by iModIntro.
   Qed.
-  
+
+
   Lemma search_spec_high N γ_te γ_he γ_s Inv_tpl γ_td γ_ght (k: K) :
   ⊢ ⌜k ∈ KS⌝ -∗ 
-      <<< ∀ t M, MCS_high N γ_te γ_he γ_s Inv_tpl γ_td γ_ght t M >>>
+      <<< ∀ M, MCS_high N γ_te γ_he γ_s Inv_tpl γ_td γ_ght M >>>
             search' #k @ ⊤ ∖ (↑(mcsN N) ∪ ↑(threadN N))
-      <<<  ∃ (vt: V*TS), MCS_high N γ_te γ_he γ_s Inv_tpl γ_td γ_ght t M 
-                        ∗ ⌜M !!! k = vt⌝, RET (#vt.1, #vt.2) >>>.
+      <<<  ∃ (v: V), MCS_high N γ_te γ_he γ_s Inv_tpl γ_td γ_ght M 
+                        ∗ ⌜M !!! k = v⌝, RET #v >>>.
   Proof.
     iIntros "%" (Φ) "AU". rename H0 into k_in_KS.
     iApply fupd_wp. 
-    iMod "AU" as (T0 M0)"[H [Hab _]]".
-    iDestruct "H" as (H0)"(MCS & M_eq_H & #HInv)".
+    iMod "AU" as (M0)"[H [Hab _]]".
+    iDestruct "H" as (T0 H0)"(MCS & M_eq_H & #HInv)".
     iMod ("Hab" with "[MCS M_eq_H]") as "AU".
-    iExists H0. iFrame "∗#". iModIntro.
+    iExists T0, H0. iFrame "∗#". iModIntro.
     awp_apply search_spec_intermediate; try done.
-    rewrite /atomic_acc /=. iMod "AU" as (T1 M1)"[H HAU]".
-    iDestruct "H" as (H1)"(MCS & M_eq_H & _)".
+    rewrite /atomic_acc /=. iMod "AU" as (M1)"[H HAU]".
+    iDestruct "H" as (T1 H1)"(MCS & M_eq_H & _)".
     iModIntro. iExists T1, H1. iFrame "MCS". iSplit.
     { iIntros "MCS". iDestruct "HAU" as "[Hab _]".
       iMod ("Hab" with "[MCS M_eq_H]") as "AU".
-      iExists H1. iFrame "∗#". by iModIntro. }
-    iIntros (tr)"(MCS & %)". rename H2 into H_k.   
+      iExists T1, H1. iFrame "∗#". by iModIntro. }
+    iIntros (vr tr)"(MCS & %)". rename H2 into H_k.   
     iDestruct "M_eq_H" as %M_eq_H.
-    iAssert (⌜M1 !!! k = tr⌝)%I as "M_k".
-    { iPureIntro. by rewrite <-M_eq_H. }
+    iAssert (⌜M1 !!! k = vr⌝)%I as "M_k".
+    { iPureIntro. rewrite <-M_eq_H. rewrite chop_ts_lookup_total.
+      rewrite H_k. by simpl. }
     iDestruct "HAU" as "[_ Hcomm]".
-    iSpecialize ("Hcomm" $! tr).
+    iSpecialize ("Hcomm" $! vr).
     iMod ("Hcomm" with "[MCS]") as "HΦ". 
-    iFrame "M_k". iExists H1. iFrame "∗#%".
+    iFrame "M_k". iExists T1, H1. iFrame "∗#%".
     by iModIntro.
   Qed.
+
+(*
+  Lemma chop_ts_lookup_total M M' k :
+    M' = chop_ts M →
+       M' !!! k = (M !!! k).1.
+  Proof.
+    intros Hm; subst M'.
+    set (P := λ (m': gmap K V) (m: gmap K (V*TS)),
+                   ∀ k, m' !!! k = (m !!! k).1).
+    apply (map_fold_ind P _ _); try done.
+    intros k0 vt m m' Hm HP. subst P.
+    intros k1. destruct (decide (k1 = k0)).
+    - subst k1. by rewrite !lookup_total_insert.
+    - rewrite !lookup_total_insert_ne; try done.
+  Qed.    
+*)
   
-  Lemma ghost_update_registered (k: K) (v: V) (T: TS) (N: namespace) 
+  Lemma ghost_update_registered (k: K) (v: V) (t: T) (N: namespace) 
                 (γ_te γ_he γ_ght: gname) 
                 (H1: gset KVT) (R: gset proph_id)  :
-        ⌜map_of_set (H1 ∪ {[k, v, T]}) !!! k = (v, T)⌝ -∗
-           MCS_auth γ_te γ_he (T+1) (H1 ∪ {[(k, v, T)]}) -∗          
+        ⌜map_of_set (H1 ∪ {[k, (v, t)]}) !!! k = (v, t)⌝ -∗
+           MCS_auth γ_te γ_he (t+1) (H1 ∪ {[(k, (v, t))]}) -∗          
       ([∗ set] t_id ∈ R, Reg N γ_te γ_he γ_ght H1 t_id) 
         ={⊤ ∖ ↑(mcsN N)}=∗ 
       ([∗ set] t_id ∈ R, Reg N γ_te γ_he γ_ght 
-                                      (H1 ∪ {[(k, v, T)]}) t_id)
-       ∗ MCS_auth γ_te γ_he (T+1) (H1 ∪ {[(k, v, T)]}).
-  Proof.
+                                      (H1 ∪ {[(k, (v, t))]}) t_id)
+       ∗ MCS_auth γ_te γ_he (t+1) (H1 ∪ {[(k, (v, t))]}).
+  Proof.  
     iIntros "H1_k MCS_auth".
     iDestruct "H1_k" as %H1_k.
-    iInduction R as [|x R' x_notin_R IH] "HInd" using set_ind_L; 
+    iInduction R as [|tid R' tid_notin_R IH] "HInd" using set_ind_L; 
       auto using big_sepS_empty'.
-    rewrite (big_sepS_delete _ ({[x]} ∪ R') x); last by set_solver.
-    rewrite (big_sepS_delete _ ({[x]} ∪ R') x); last by set_solver.
-    assert (({[x]} ∪ R') ∖ {[x]} = R') as HR'. set_solver.
+    rewrite (big_sepS_delete _ ({[tid]} ∪ R') tid); last by set_solver.
+    rewrite (big_sepS_delete _ ({[tid]} ∪ R') tid); last by set_solver.
+    assert (({[tid]} ∪ R') ∖ {[tid]} = R') as HR'. set_solver.
     rewrite HR'.
-    iIntros "(Hx & Hbigstar)". 
+    iIntros "(Htid & Hbigstar)". 
     iMod ("HInd" with "[$MCS_auth] Hbigstar") as "(H' & MCS_auth)".
     iFrame "H'".
-    iDestruct "Hx" as (P Q k' vtp vt γ_tk γ_sy)
+    iDestruct "Htid" as (P Q k' vp t0 vtid γ_tk γ_sy)
               "(Hreg_proph & Hreg_gh & Hreg_sy & #Pau & #Hthinv)".
     iInv "Hthinv" as (H1')"Hstate".
     iDestruct "Hstate" as "(>Hth_sy & Hstate)".
@@ -359,7 +353,7 @@ Section multicopy_client_level.
     iEval (rewrite <-frac_agree_op) in "H'". 
     iEval (rewrite Qp_half_half) in "H'".
     iMod ((own_update (γ_sy) (to_frac_agree 1 H1) 
-                  (to_frac_agree 1 (H1 ∪ {[(k, v, T)]}))) with "[$H']") as "H'".
+                  (to_frac_agree 1 (H1 ∪ {[(k, (v, t))]}))) with "[$H']") as "H'".
     { apply cmra_update_exclusive. 
       unfold valid, cmra_valid. simpl. unfold prod_valid_instance.
       split; simpl; try done. }
@@ -369,58 +363,88 @@ Section multicopy_client_level.
 
     iDestruct "Hstate" as "[Hpending | Hdone]".
     - iDestruct "Hpending" as "(P & >%)".
-      rename H0 into vp_notin_H.
-      destruct (decide ((k', vtp.1, vtp.2) ∈ H1 ∪ {[(k, v, T)]})).
-      + assert ((k',vtp.1, vtp.2) = (k, v, T)) as H'. 
-        { clear -vp_notin_H e. set_solver. }
-        inversion H'. subst k'. rename H3 into Hv; rename H4 into Ht. 
-        rewrite Hv Ht.
-        iDestruct ("Pau" with "P") as ">AU".
-        iMod "AU" as (t H1')"[MCS [_ Hclose]]". set_solver.
-        iAssert (⌜H1' = H1 ∪ {[(k, v, T)]}⌝)%I as "%".
-        { iPoseProof (MCS_agree with "[$MCS_auth] [$MCS]") as "(% & %)".
-          by iPureIntro. } subst H1'.
-        iSpecialize ("Hclose" $! (v,T)).  
-        iMod ("Hclose" with "[MCS]") as "HQ".
-        { iFrame "%∗". }
-        iModIntro. iSplitL "Hth_sy HQ".
-        iNext. iExists (H1 ∪ {[(k, v, T)]}). iFrame.
-        iRight. iSplitL. iLeft. rewrite Hv Ht.
-        by iEval (simpl) in "HQ".
-        iPureIntro. rewrite Hv Ht. clear; set_solver.
-        iModIntro. iFrame.
-        iExists P, Q, k, vtp, vt, γ_tk, γ_sy.
-        iFrame "∗#".
-      + iModIntro. iSplitR "Hreg_proph Hreg_sy Hreg_gh MCS_auth".
-        iNext. iExists (H1 ∪ {[(k, v, T)]}). iFrame.
-        iLeft. iFrame. by iPureIntro.
-        iModIntro. iFrame.             
-        iExists P, Q, k', vtp, vt, γ_tk, γ_sy.
-        iFrame "∗#".
+      rename H0 into HPending.
+      destruct (decide (k' = k)).
+      + subst k'. destruct (decide (vp = v)).
+        * subst vp. 
+          assert (t0 ≤ t ∨ t < t0) as H'.
+          { clear; lia. }
+          destruct H' as [H' | H'].
+          ** iDestruct ("Pau" with "P") as ">AU".
+             iMod "AU" as (t' H1')"[MCS [_ Hclose]]". set_solver.
+             iAssert (⌜H1' = H1 ∪ {[(k, (v, t))]}⌝)%I as "%".
+             { iPoseProof (MCS_agree with "[$MCS_auth] [$MCS]") as "(% & %)".
+               by iPureIntro. } subst H1'.
+             iSpecialize ("Hclose" $! v t).  
+             iMod ("Hclose" with "[MCS]") as "HQ".
+             { iFrame "%∗". }
+             iModIntro. iSplitL "Hth_sy HQ".
+             *** iNext. iExists (H1 ∪ {[(k, (v, t))]}).
+                 iFrame. iRight. unfold Done. iSplitL.
+                 iLeft. iFrame.
+                 iPureIntro. exists t.
+                 split. clear; set_solver. lia.
+             *** iModIntro. iFrame.
+                 iExists P, Q, k, v, t0, vtid, γ_tk, γ_sy.
+                 iFrame "∗#".
+          ** iModIntro. iSplitL "Hth_sy P".
+             *** iNext. iExists (H1 ∪ {[(k, (v, t))]}).
+                 iFrame. iLeft. iFrame.
+                 iPureIntro. intros t'.
+                 rewrite elem_of_union.
+                 intros [H'' | H''].
+                 by apply HPending.
+                 assert (t' = t) by set_solver.
+                 subst t'. done.
+             *** iModIntro. iFrame.
+                 iExists P, Q, k, v, t0, vtid, γ_tk, γ_sy.
+                 iFrame "∗#".
+        * iModIntro. iSplitL "Hth_sy P".
+          ** iNext. iExists (H1 ∪ {[(k, (v, t))]}).
+             iFrame. iLeft. iFrame.
+             iPureIntro. intros t'.
+             rewrite elem_of_union.
+             intros [H'' | H''].
+             by apply HPending.
+             assert (vp = v) by set_solver.
+             done.
+          ** iModIntro. iFrame.
+             iExists P, Q, k, vp, t0, vtid, γ_tk, γ_sy.
+             iFrame "∗#".
+      + iModIntro. iSplitL "Hth_sy P".
+        * iNext. iExists (H1 ∪ {[(k, (v, t))]}).
+          iFrame. iLeft. iFrame.
+          iPureIntro. intros t'.
+          rewrite elem_of_union.
+          intros [H'' | H''].
+          by apply HPending.
+          assert (k' = k) by set_solver.
+          done.
+        * iModIntro. iFrame.
+          iExists P, Q, k', vp, t0, vtid, γ_tk, γ_sy.
+          iFrame "∗#".                
     - iModIntro.
       iSplitR "Hreg_proph Hreg_sy Hreg_gh MCS_auth".
-      iNext. iExists (H1 ∪ {[(k, v, T)]}). iFrame.
+      iNext. iExists (H1 ∪ {[(k, (v, t))]}). iFrame.
       iRight. iDestruct "Hdone" as "(HQ & %)".
       iFrame "HQ". iPureIntro. set_solver.
       iModIntro. iFrame. 
-      iExists P, Q, k', vtp, vt, γ_tk, γ_sy.
-      iFrame "∗#". 
-  Qed.  
-  
+      iExists P, Q, k', vp, t0, vtid, γ_tk, γ_sy.
+      iFrame "∗#".                     
+  Qed.
   
   Lemma upsert_spec_high N γ_te γ_he γ_s Inv_tpl γ_td γ_ght (k: K) (v: V):
     ⊢ ⌜k ∈ KS⌝ -∗ 
-            <<< ∀ T M, MCS_high N γ_te γ_he γ_s Inv_tpl γ_td γ_ght T M >>> 
-                   upsert #k #v @ ⊤ ∖ (↑(mcsN N) ∪ ↑(threadN N))
-            <<< MCS_high N γ_te γ_he γ_s Inv_tpl γ_td γ_ght 
-                        (T + 1) (<[k := (v,T)]> M), RET #() >>>.
+       <<< ∀ M, MCS_high N γ_te γ_he γ_s Inv_tpl γ_td γ_ght M >>> 
+             upsert #k #v @ ⊤ ∖ (↑(mcsN N) ∪ ↑(threadN N))
+       <<< MCS_high N γ_te γ_he γ_s Inv_tpl γ_td γ_ght (<[k := v]> M), RET #() >>>.
   Proof.
     iIntros "%" (Φ) "AU". rename H0 into k_in_KS.
     iApply fupd_wp. 
-    iMod "AU" as (T0 M0)"[H [Hab _]]".
-    iDestruct "H" as (H0)"(MCS & M_eq_H & #HInv)".
+    iMod "AU" as (M0)"[H [Hab _]]".
+    iDestruct "H" as (T0 H0)"(MCS & M_eq_H & #HInv)".
     iMod ("Hab" with "[MCS M_eq_H]") as "AU".
-    iExists H0. iFrame "∗#". iModIntro.
+    iExists T0, H0. iFrame "∗#". iModIntro.
     iAssert (ghost_update_protocol N γ_te γ_he 
                 (Prot_help N γ_te γ_he γ_td γ_ght) k)%I 
                   as "Ghost_updP".
@@ -435,23 +459,24 @@ Section multicopy_client_level.
       iExists R, hγt. iFrame. }
     awp_apply upsert_spec; try done.
     iApply (aacc_aupd_commit with "AU"). set_solver.
-    iIntros (T1 M1)"MCS_high".
-    iDestruct "MCS_high" as (H1)"(MCS & M_eq_H & _)".
+    iIntros (M1)"MCS_high".
+    iDestruct "MCS_high" as (T1 H1)"(MCS & M_eq_H & _)".
     iDestruct "M_eq_H" as %M_eq_H.
-    iAssert (⌜maxTS T1 H1⌝)%I as %maxTS.
+    iAssert (⌜HClock T1 H1⌝)%I as %HClock.
     { by iDestruct "MCS" as "(_ & _ & % & _)". }
-    iAssert (⌜unique_val H1⌝)%I as %Uniq.
+    iAssert (⌜HUnique H1⌝)%I as %HUniq.
     { by iDestruct "MCS" as "(_ & _ & _ & %)". }
     iAaccIntro with "MCS".
     { iIntros "MCS". iModIntro.
       iSplitL; try eauto with iFrame.
-      iExists H1; iFrame "∗#%". } 
+      iExists T1, H1; iFrame "∗#%". } 
     iIntros "MCS". 
     iModIntro. iSplitL.
-    iExists (H1 ∪ {[k, v, T1]}). iFrame "∗#".
-    { iPureIntro. apply symmetry. 
-      apply map_of_set_insert_eq; try done.
-      apply maxTS. }
+    iExists (T1 + 1), (H1 ∪ {[(k, (v, T1))]}). iFrame "∗#".
+    { iPureIntro. apply symmetry.
+      pose proof map_of_set_insert_eq k v T1 H1 HUniq HClock as H'.
+      apply symmetry in H'. rewrite H'. rewrite <-M_eq_H.
+      by rewrite chop_ts_insert. }
     iIntros "HΦ"; iModIntro; try done.
   Qed.
               
