templates/multicopy/multicopy_lsm_upsert.v
@@ -14,129 +14,111 @@ Section multicopy_lsm_upsert.
   Notation iProp := (iProp Σ).
   Local Notation "m !1 i" := (nzmap_total_lookup i m) (at level 20).
   
-  Lemma upsert_spec N γ_te γ_he γ_s Prot γ_t γ_I γ_J γ_f γ_gh lc r (k: K) :
+  Lemma upsert_spec N γ_te γ_he γ_s Prot γ_I γ_J γ_f γ_gh r (k: K) (v: V) :
     ⊢ ⌜k ∈ KS⌝ -∗ 
         (ghost_update_protocol N γ_te γ_he Prot k) -∗ 
         mcs_inv N γ_te γ_he γ_s Prot 
-          (Inv_LSM γ_s γ_t γ_I γ_J γ_f γ_gh lc r) -∗
+          (Inv_LSM γ_s γ_I γ_J γ_f γ_gh r) -∗
             <<< ∀ t H, MCS γ_te γ_he t H >>> 
-                   upsert lc r #k @ ⊤ ∖ (↑(mcsN N))
-            <<< MCS γ_te γ_he (t + 1) (H ∪ {[(k,t)]}), RET #() >>>.
+                   upsert r #k #v @ ⊤ ∖ (↑(mcsN N))
+            <<< MCS γ_te γ_he (t + 1) (H ∪ {[(k, (v, t))]}), RET #() >>>.
   Proof.
     iIntros "%". iLöb as "IH".
     rename H into k_in_KS.    
-    iIntros "Ghost_updP #HInv" (Φ) "AU". wp_lam.
+    iIntros "Ghost_updP #HInv" (Φ) "AU". wp_lam. wp_pures.
     iApply fupd_wp. 
     (** Open invariant to establish root node in footprint **)
-    iInv "HInv" as (T0 H0)"(mcs_high & >Inv_LSM)".
+    iInv "HInv" as (t0 H0)"(mcs_high & >Inv_LSM)".
     iDestruct "Inv_LSM" as (hγ0 I0 J0)"(Hglob & Hstar)".
-    iDestruct "Hglob" as "(Ht & HI & Out_I & HR 
+    iDestruct "Hglob" as "(HI & Out_I & HR 
             & Out_J & Inf_J & Hf & Hγ & #FP_r & domm_IR & domm_Iγ)".
     iModIntro. iSplitR "AU Ghost_updP". iNext. 
-    iExists T0, H0. iFrame "mcs_high". 
+    iExists t0, H0. iFrame "mcs_high". 
     iExists hγ0, I0, J0. iFrame "∗ #". iModIntro.
     (** Lock the node r **)
     awp_apply lockNode_spec_high without "Ghost_updP"; try done.
     iAaccIntro with ""; try eauto with iFrame. 
     iIntros (Cr Qr)"HnP_n". iModIntro. 
     iIntros "Ghost_updP". wp_pures.
-    iDestruct "HnP_n" as (γ_er γ_cr γ_qr γ_cirr es T)
-                      "(node_r & #HnP_gh & HnP_frac & HnP_C & HnP_t)".
-    iEval (rewrite decide_True) in "HnP_t".
-    wp_apply (readClock_spec with "[HnP_t]"); try done.
-    iIntros "HnP_t". wp_pures.
+    iDestruct "HnP_n" as (γ_er γ_cr γ_qr γ_cirr es Vr Tr)
+                      "(node_r & #HnP_gh & HnP_frac & HnP_C & HnP_cts)".
     wp_apply (addContents_spec with "[$node_r]"); try done.
-    iIntros (b Cr')"(node_r & Hif)".
+    iIntros (b Vr')"(node_r & Hif)".
     (** Case analysis on whether addContents is successful **)
     destruct b; last first.
     - (** Case : addContents fails. Unlock root node and apply 
                  inductive hypothesis IH **) 
-      iDestruct "Hif" as %HCr. replace Cr'. wp_pures.
+      iDestruct "Hif" as %HVr. replace Vr'. wp_pures.
       awp_apply (unlockNode_spec_high 
-          with "[] [] [HnP_gh HnP_frac HnP_C HnP_t node_r]") 
+          with "[] [] [HnP_gh HnP_frac HnP_C HnP_cts node_r]") 
             without "Ghost_updP" ; try done.
-      { iExists γ_er, γ_cr, γ_qr, γ_cirr, es, T.
-        iFrame "∗#". iEval (rewrite decide_True); try done. }
+      { iExists γ_er, γ_cr, γ_qr, γ_cirr, es, Vr, Tr.
+        iFrame "∗#". }
       iAaccIntro with ""; try eauto with iFrame.
       iIntros "_". iModIntro.
       iIntros "Ghost_updP". wp_pures.
       iApply ("IH" with "Ghost_updP"); try done.
     - (** Case : addContent successful **)
       (** Linearization Point: open invariant and update the resources **)
-      wp_pures. wp_bind (incrementClock _)%E.
-      wp_lam. iDestruct "HnP_t" as "(HnP_T & HnP_lc)".
-      unfold clock. wp_load. wp_pures. 
-      iInv "HInv" as (T1 H1)"(mcs_high & >Inv_LSM)".
+      wp_pures. iApply fupd_wp.
+      iInv "HInv" as (t1 H1)"(mcs_high & >Inv_LSM)".
       iDestruct "Inv_LSM" as (hγ1 I1 J1)"(Hglob & Hstar)".
-      iDestruct "mcs_high" as "(>MCS_auth & >HH & >Hist & >MaxTS & Prot)".
-      iDestruct "Hglob" as "(Ht & HI & Out_I & HR 
+      iDestruct "mcs_high" as "(>MCS_auth & >HH & >HInit & >HClock & >HUniq & Prot)".
+      iDestruct "Hglob" as "(HI & Out_I & HR 
             & Out_J & Inf_J & Hf & Hγ & _ & domm_IR & domm_Iγ)".
-      wp_store. 
       
-      iDestruct "Hif" as %HCr.
-      iAssert (⌜T = T1⌝)%I as %HT. 
-      { iPoseProof ((own_valid_2 _ _ _) with "[$HnP_T] [$Ht]") as "H'".
-        iDestruct "H'" as %H'. 
-        pose proof (auth_auth_frac_op_inv _ _ _ _ H') as H''.
-        inversion H''. by iPureIntro. } replace T1.
-      iCombine "Ht HnP_T" as "HT".  
-      iMod (own_update (γ_t) (● (MaxNat (T))) 
-               (● (MaxNat (T+1))) with "HT") as "HT".
-      { apply (auth_update_auth _ _ (MaxNat (T+1))).
-        apply max_nat_local_update. simpl. lia. }
-      iDestruct "HT" as "(Ht & HnP_T)".  
-
-      iAssert (own γ_t (●{1 / 2} MaxNat (T + 1)) ∗ clock lc (T + 1))%I
-        with "[HnP_T HnP_lc]" as "HnP_t".
-      { iFrame "HnP_T". unfold clock.
-        assert (#(T+1)%nat = #(T+1)) as H'.
-        apply f_equal. apply f_equal. lia. 
-        by rewrite H'. }  
-
+      iDestruct "Hif" as %HVr'.
+      
+      set (Tr' := <[k := t1]> Tr).
+      set (Cr' := <[k := (v, t1)]> Cr).
+      set (H1' := H1 ∪ {[(k, (v, t1))]}).
+      
       iPoseProof ((auth_own_incl γ_s H1 _) with "[$HH $HnP_C]") as "%".
       rename H into Cr_sub_H1. apply gset_included in Cr_sub_H1.
-      iDestruct "MaxTS" as %MaxTS_H1.
+      iDestruct "HClock" as %HClock_H1.
       (** Re-establish maxTS for updated T and H **)
-      assert (maxTS (T+1) (H1 ∪ {[(k, T)]})) as Max_ts.
-      { split. intros k' t' H.
-        assert (((k',t') ∈ H1) ∨ (k' = k ∧ t' = T)) as Hor by set_solver.
+      assert (HClock (t1 + 1) H1') as HClock_H1'.
+      { subst H1'. intros k' v' t' H'.
+        assert (((k', (v', t')) ∈ H1) ∨ (k' = k ∧ v' = v ∧ t' = t1)) 
+              as Hor by set_solver.
         destruct Hor as [Hor | Hor]. 
-        destruct MaxTS_H1 as [MaxTS_H1 _].
-        pose proof MaxTS_H1 k' t' Hor as Hres. lia.
-        destruct Hor as [_ Hor]. replace t'. lia.
-        destruct MaxTS_H1 as [_ MaxTS_H1]. lia. }       
-      iAssert (⌜set_of_map Cr' ⊆ H1 ∪ {[(k,T)]}⌝)%I as %Cr_sub_H1'.
-      { iPureIntro. replace Cr'.
-        pose proof (set_of_map_insert_subseteq Cr k T) as H'.
+        pose proof HClock_H1 k' v' t' Hor as Hres. lia.
+        destruct Hor as [_ [_ Hor]]. replace t'. lia. }       
+      iAssert (⌜set_of_map Cr' ⊆ H1'⌝)%I as %Cr'_sub_H1'.
+      { subst H1'. iPureIntro. subst Cr'.
+        pose proof (set_of_map_insert_subseteq Cr k v t1) as H'.
         assert (set_of_map Cr = set_of_map Cr) as H'' by done. 
         set_solver. }
       (** Update the (● H) resource **)  
-      iMod (own_update γ_s (● H1) (● (H1 ∪ {[(k,T)]})) with "[$HH]") as "HH".
-      { apply (auth_update_auth _ _ (H1 ∪ {[(k,T)]})).
+      iMod (own_update γ_s (● H1) (● H1') 
+          with "[$HH]") as "HH".
+      { apply (auth_update_auth _ _ H1').
         apply gset_local_update. set_solver. }
-      iMod (own_update γ_s (● (H1 ∪ {[(k, T)]})) 
-             (● (H1 ∪ {[(k, T)]}) ⋅ ◯ (set_of_map Cr')) with "[$HH]") as "HH".
-      { apply (auth_update_alloc _ (H1 ∪ {[(k,T)]}) (set_of_map Cr')).
+      iMod (own_update γ_s (● H1') 
+             (● H1' ⋅ ◯ (set_of_map Cr')) 
+              with "[$HH]") as "HH".
+      { subst H1'.
+        apply (auth_update_alloc _ (H1 ∪ {[(k, (v, t1))]}) (set_of_map Cr')).
         apply local_update_discrete. intros m Valid_H1 H1_eq.
         split; try done. rewrite /(ε ⋅? m) in H1_eq.
         destruct m. rewrite gset_op in H1_eq. 
         rewrite left_id in H1_eq *; intros H1_eq.
         rewrite <-H1_eq. 
-        rewrite /(set_of_map Cr' ⋅? Some (H1 ∪ {[k, T]})).
+        rewrite /(set_of_map Cr' ⋅? Some (H1 ∪ {[k, (v, t1)]})).
         rewrite gset_op.
         rewrite /(ε) in H1_eq. unfold ucmra_unit in H1_eq.
         simpl in H1_eq.
-        assert ((k,T) ∈ set_of_map Cr') as H'.
-        { replace Cr'. apply set_of_map_member.
+        assert ((k, (v, t1)) ∈ set_of_map Cr') as H'.
+        { subst Cr'. apply set_of_map_member.
           apply lookup_insert. } 
-        clear - H' Cr_sub_H1 Cr_sub_H1'. set_solver.
+        clear - H' Cr_sub_H1 Cr'_sub_H1'. set_solver.
         exfalso. clear -H1_eq. set_solver. }
       (** Re-establish history_init **)   
-      iAssert (⌜init (H1 ∪ {[(k, T)]})⌝)%I with "[Hist]" as "Hist".
-      { iDestruct "Hist" as %Hist.
-        unfold init. iPureIntro.
-        clear -Hist k_in_KS. intros k' Hk'.
-        pose proof Hist k' Hk' as H'. set_solver. }  
+      iAssert (⌜HInit H1'⌝)%I with "[HInit]" as "HInit".
+      { subst H1'. iDestruct "HInit" as %HInit.
+        unfold multicopy.HInit. iPureIntro.
+        clear -HInit k_in_KS. intros k' Hk'.
+        pose proof HInit k' Hk' as H'. set_solver. }  
       iDestruct "HnP_C" as "_".  
       iDestruct "HH" as "(HH & HnP_C)".   
       iAssert (⌜r ∈ domm I1⌝)%I as %r_in_I.
@@ -146,54 +128,58 @@ Section multicopy_lsm_upsert.
       iDestruct "H_r" as (br Cr'' Qr'')"(Hl_r & HnS_r)".
       iPoseProof (nodePred_lockR_true with "[$node_r] [$Hl_r]")
          as "%". subst br.
-      iDestruct "HnS_r" as (γ_er' γ_cr' γ_qr' γ_cirr' es' Br Ir Jr) "HnS_r'".
+      iDestruct "HnS_r" as (γ_er' γ_cr' γ_qr' γ_cirr' es' Tr'' Br Ir Jr) "HnS_r'".
       iPoseProof (nodePred_nodeShared_eq with "[$HnP_gh] [$HnP_frac] [$HnS_r']")
-           as "(HnP_frac & HnS_r' &%&%&%)". subst es' Cr'' Qr''.   
+           as "(HnP_frac & HnS_r' &%&%&%)". subst es' Tr'' Qr''.   
       iDestruct "HnS_r'" as "(HnS_gh & HnS_frac & HnS_si & HnS_FP 
                             & HnS_cl & HnS_oc & HnS_Bn & HnS_H & HnS_star & Hφ)".
 
 
       (** Update contents-in-reach of r **)
-      set (Br' := <[k := T]>Br).
-      assert (Br' = <[k := T]>Br) as HBr'. try done.
+      set (Br' := <[k := t1]>Br).
+      assert (Br' = <[k := t1]>Br) as HBr'. try done.
       iEval (rewrite decide_True) in "HnS_H".
       iDestruct "HnS_H" as "(% & %)". 
       rename H into Br_eq_H1. rename H2 into Infz_Ir.
 
-      iAssert (⌜contents_in_reach Br' Cr' Qr⌝)%I with "[HnS_Bn]" as "HnS_Bn".
+      iAssert (⌜contents_in_reach Br' Tr' Qr⌝)%I with "[HnS_Bn]" as "HnS_Bn".
       { iDestruct "HnS_Bn" as %H'. iPureIntro. 
-        intros k0 t0 HKS. destruct (decide (k0 = k)).
-        - subst k0. subst Cr' Br'.
+        intros k' t' HKS. destruct (decide (k' = k)).
+        - subst k'. subst Tr' Br'.
           rewrite !lookup_insert.
           split; try done.
-        - subst Cr' Br'. 
+        - subst Tr' Br'. 
           rewrite !lookup_insert_ne; try done.
-          pose proof H' k0 t0 HKS; try done. }
+          pose proof H' k' t' HKS; try done. }
 
       
-      iAssert (⌜Br' = map_of_set (H1 ∪ {[(k, T)]})⌝)%I as %Br'_eq_H1.
-      { iPureIntro.
-        apply map_of_set_insert_eq; try done.
-        intros t. 
-        destruct MaxTS_H1 as [MaxTS_H1 _].
-        by pose proof MaxTS_H1 k t. }
+      iAssert (⌜∀ k : K, Br' !!! k = (map_of_set H1' !!! k).2⌝)%I as %Br'_eq_H1'.
+      { iDestruct "HUniq" as %HUniq. 
+        iPureIntro. subst Br' H1'. intros k'.
+        rewrite <-map_of_set_insert_eq; try done.
+        destruct (decide (k' = k)).
+        - subst k'. rewrite !lookup_total_insert; by simpl.
+        - rewrite !lookup_total_insert_ne; try done. }
       iEval (rewrite (big_sepS_delete (_) (KS) k); last by eauto) in "HnS_star".
       iDestruct "HnS_star" as "(Hk & HnS_star')".
-      iAssert (⌜Br !!! k ≤ T⌝)%I as %Br_le_T. 
+      iAssert (⌜Br !!! k ≤ t1⌝)%I as %Br_le_t1. 
       { iPureIntro. rewrite lookup_total_alt.
         destruct (Br !! k) eqn: Hbrk; last first.
         - rewrite Hbrk. simpl; clear; lia.
-        - rewrite Hbrk. simpl. 
-          rewrite Br_eq_H1 in Hbrk.
+        - rewrite Hbrk. simpl.
+          pose proof Br_eq_H1 k as Br_eq_H1. 
+          (* rewrite Br_eq_H1 in Hbrk. *)
           pose proof map_of_set_lookup_cases H1 k as H'.
           destruct H' as [H' | [_ H']]; last first.
-          + rewrite H' in Hbrk. inversion Hbrk.
-          + destruct H' as [Tk [H' [_ H'']]].
-            rewrite H'' in Hbrk. inversion Hbrk.
-            subst Tk.
-            destruct MaxTS_H1 as [MaxTS_H1 _].
-            pose proof MaxTS_H1 k u H' as H'''.
-            clear -H'''; lia. }  
+          + rewrite !lookup_total_alt in Br_eq_H1.
+            rewrite H' Hbrk in Br_eq_H1. simpl in Br_eq_H1. 
+            subst t; clear; lia.
+          + destruct H' as [v' [t' [H' [H'' H''']]]].
+            rewrite !lookup_total_alt in Br_eq_H1.
+            rewrite H''' Hbrk in Br_eq_H1. simpl in Br_eq_H1.
+            subst t'. 
+            pose proof HClock_H1 k v' t H' as H''''.
+            clear -H''''; lia. }  
       iMod (own_update (γ_cirr !!! k) (● (MaxNat (Br !!! k))) 
                 (● (MaxNat (Br' !!! k))) with "Hk") as "Hk".
       { apply (auth_update_auth _ _ (MaxNat (Br' !!! k))).
@@ -212,15 +198,15 @@ Section multicopy_lsm_upsert.
         intros x Hx. assert (x ≠ k) as H' by set_solver.
         iFrame. iSplit. 
         iIntros "H". iEval (rewrite HBr') in "H".
-        assert (<[k:=T]> Br !!! x = Br !!! x) as H''. 
+        assert (<[k := t1]> Br !!! x = Br !!! x) as H''. 
         { apply lookup_total_insert_ne; try done. } 
         by iEval (rewrite H'') in "H".       
         iIntros "H". iEval (rewrite HBr').
-        assert (<[k:=T]> Br !!! x = Br !!! x) as H''. 
+        assert (<[k:= t1]> Br !!! x = Br !!! x) as H''. 
         { apply lookup_total_insert_ne; try done. } 
         by iEval (rewrite H'').
         done. }
-      iMod ((frac_update γ_er γ_cr γ_qr es Cr Qr es Cr' Qr) 
+      iMod ((frac_update γ_er γ_cr γ_qr es Tr Qr es Tr' Qr) 
                   with "[$HnP_frac $HnS_frac]") as "(HnP_frac & HnS_frac)".
       iDestruct "Inf_J" as %Inf_J.
       iPoseProof ((auth_own_incl γ_J J1 Jr) with "[HR HnS_si]")
@@ -257,17 +243,53 @@ Section multicopy_lsm_upsert.
           by rewrite decide_True in Inf_J.
           rewrite Domm_Jr. clear. set_solver. }
             
+      iAssert (⌜HUnique H1'⌝)%I with "[HUniq]" as %HUniq.
+      { iDestruct "HUniq" as %HUniq.
+        iPureIntro. subst H1'.
+        intros k' t' v' v'' H' H''.
+        assert (((k', (v', t')) ∈ H1) ∨ (k' = k ∧ v' = v ∧ t' = t1)) 
+              as Hor by set_solver.
+        assert (((k', (v'', t')) ∈ H1) ∨ (k' = k ∧ v'' = v ∧ t' = t1)) 
+              as Hor' by set_solver.
+        destruct Hor as [Hor | Hor]. 
+        - destruct Hor' as [Hor' | Hor'].
+          + apply (HUniq k' t' v' v'' Hor Hor'); try done.
+          + destruct Hor' as [? [? ?]]. subst k' v'' t'.
+            apply (HClock_H1 k v' t1) in Hor.
+            clear -Hor; lia.
+        - destruct Hor as [? [? ?]]. subst k' v' t'.
+          destruct Hor' as [Hor' | Hor'].
+          + apply (HClock_H1 k v'' t1) in Hor'.
+            clear -Hor'; lia.
+          + destruct Hor' as [? [? ?]]. by subst v''. }  
+          
+      iAssert (contents_proj Cr' Vr' Tr')%I with "[HnP_cts]" as "HnP_cts".
+      { iDestruct "HnP_cts" as "(% & % & %)".
+        rename H into dom_Cr_Vr; rename H2 into dom_Cr_Tr;
+        rename H3 into Cr_eq_Vr_Tr. 
+        iPureIntro. subst Cr' Vr' Tr'. split; last split.
+        - apply leibniz_equiv. rewrite !dom_insert.
+          rewrite dom_Cr_Vr. clear; set_solver.
+        - apply leibniz_equiv. rewrite !dom_insert.
+          rewrite dom_Cr_Tr. clear; set_solver.
+        - intros k' v' t'. destruct (decide (k' = k)).
+          + subst k'. rewrite !lookup_insert. split.
+            * intros H'; by inversion H'.
+            * intros [H' H'']; inversion H'; by inversion H''.
+          + rewrite !lookup_insert_ne; try done. }
+        
+          
             
       (** Linearization **)    
-      iMod "AU" as (t' H1')"[MCS [_ Hclose]]".
-      iAssert (⌜t' = T ∧ H1' = H1⌝)%I as "(% & %)". 
+      iMod "AU" as (t' H1'')"[MCS [_ Hclose]]".
+      iAssert (⌜t' = t1 ∧ H1'' = H1⌝)%I as "(% & %)". 
       { iPoseProof (MCS_agree with "[$MCS_auth] [$MCS]") as "(% & %)".
-        by iPureIntro. } subst t' H1'. 
+        by iPureIntro. } subst t' H1''. 
       iDestruct "MCS" as "(MCS◯t & MCS◯h & _)".
       iDestruct "MCS_auth" as "(MCS●t & MCS●h)".
-      iMod ((auth_excl_update γ_te (T+1) T T) with "MCS●t MCS◯t") 
+      iMod ((auth_excl_update γ_te (t1+1) t1 t1) with "MCS●t MCS◯t") 
                                           as "(MCS●t & MCS◯t)".
-      iMod ((auth_excl_update γ_he (H1 ∪ {[(k, T)]}) H1 H1) with "MCS●h MCS◯h") 
+      iMod ((auth_excl_update γ_he (H1 ∪ {[(k, (v, t1))]}) H1 H1) with "MCS●h MCS◯h") 
                                           as "(MCS●h & MCS◯h)".
       iCombine "MCS◯t MCS◯h" as "(MCS_t & MCS_h)".
       iCombine "MCS●t MCS●h" as "MCS_auth".
@@ -275,10 +297,13 @@ Section multicopy_lsm_upsert.
       iFrame. by iPureIntro.
       
       (** Use ghost_update_protocol to update Prot(H) **)
-      iSpecialize ("Ghost_updP" $! T H1).
+      iSpecialize ("Ghost_updP" $! v t1 H1).
+
+(*      
       iMod ("Ghost_updP" with "[] [$MCS_auth] [$Prot]") 
                         as "(Prot & MCS_auth)". 
-      { pose proof map_of_set_lookup (H1 ∪ {[k, T]}) k T as H'.
+      { assert ((k, (v, t1)) ∈ H1') as H' by set_solver.
+        pose proof map_of_set_lookup H1' k v t1 HUniq H' as H''.
         iPureIntro. rewrite lookup_total_alt.
         rewrite H'. by simpl. clear; set_solver.
         intros t. rewrite elem_of_union.
@@ -287,45 +312,46 @@ Section multicopy_lsm_upsert.
         pose proof MaxTS_H1 k t H' as H''; clear -H''; lia.
         rewrite elem_of_singleton in H'*; intros H'.
         inversion H'. lia. }          
+*)
             
       iModIntro.
-      iSplitR "HΦ node_r HnP_t HnP_C HnP_frac".
-      { iNext. iExists (T+1), (H1 ∪ {[(k, T)]}). iFrame "∗".
-        iSplitR; first by iPureIntro.
+      iSplitR "HΦ node_r HnP_cts HnP_C HnP_frac".
+      { iNext. iExists (t1+1), (H1 ∪ {[(k, (v, t1))]}). iFrame "∗".
+        iSplitL "Prot". repeat (iSplitR; first by iPureIntro).
+        admit.
         iExists hγ1, I1, J1. iFrame "∗ %".   
         rewrite (big_sepS_delete _ (domm I1) r); last by eauto.
         iSplitR "Hstar'".
-        { iExists true, Cr', Qr. iFrame.
-          iExists γ_er, γ_cr, γ_qr, γ_cirr, es, Br', Ir, Jr.
+        { iExists true, Cr'', Qr. iFrame.
+          iExists γ_er, γ_cr, γ_qr, γ_cirr, es, Tr', Br', Ir. iExists Jr.
           iFrame "∗#". iEval (rewrite decide_True). 
           iFrame "%∗". }        
         iApply (big_sepS_mono 
-                  (λ y, ∃ (bn : bool) (Cn Qn : gmap K natUR),
-                          lockR bn y (nodePred γ_gh γ_t γ_s lc r y Cn Qn)
-                        ∗ nodeShared γ_I γ_J γ_f γ_gh r y Cn Qn H1)%I
-                  (λ y, ∃ (bn : bool) (Cn Qn : gmap K natUR),
-                          lockR bn y (nodePred γ_gh γ_t γ_s lc r y Cn Qn)
-                        ∗ nodeShared γ_I γ_J γ_f γ_gh r y Cn Qn 
-                                                (H1 ∪ {[(k, T)]}))%I
+                  (λ y, ∃ (bn : bool) (Cn : gmap K (V * T)) (Qn : gmap K T),
+                          lockR bn y (nodePred γ_gh γ_s r y Cn Qn)
+                        ∗ nodeShared γ_I γ_J γ_f γ_gh r y Qn H1)%I
+                  (λ y, ∃ (bn : bool) (Cn : gmap K (V * T)) (Qn : gmap K T),
+                          lockR bn y (nodePred γ_gh γ_s r y Cn Qn)
+                        ∗ nodeShared γ_I γ_J γ_f γ_gh r y Qn (H1 ∪ {[k, (v, t1)]}))%I
                   (domm I1 ∖ {[r]})); try done.
         intros y y_dom. assert (y ≠ r) as Hy by set_solver. iFrame.
         iIntros "Hstar". iDestruct "Hstar" as (b C Q)"(Hl & HnS)".
         iExists b, C, Q. iFrame. 
-        iDestruct "HnS" as (γ_e γ_c γ_q γ_cir esy By Iy Ry)
+        iDestruct "HnS" as (γ_e γ_c γ_q γ_cir esy Ty By Iy Jy)
                     "(HnS_gh & domm_γcir & HnS_frac & HnS_si & HnS_FP 
                               & HnS_cl & HnS_oc & HnS_Bn & HnS_H & HnS_star 
                               & Hφ0 & Hφ2 & Hφ3 & Hφ4 & Hφ5 & Hφ7)".
-        iExists γ_e, γ_c, γ_q, γ_cir, esy, By, Iy, Ry. iFrame.
+        iExists γ_e, γ_c, γ_q, γ_cir, esy, Ty, By, Iy. iExists Jy. iFrame.
         destruct (decide (y = r)); try done. } 
-      wp_pures. 
+      iModIntro. 
       (** Unlock node r **) 
       awp_apply (unlockNode_spec_high with "[] [] 
-        [HnP_t HnP_C HnP_frac node_r]") without "HΦ"; try done.   
-      iExists γ_er, γ_cr, γ_qr, γ_cirr, es, (T + 1).
-      iFrame "∗#". by iEval (rewrite decide_True).
+        [HnP_cts HnP_C HnP_frac node_r]") without "HΦ"; try done.   
+      iExists γ_er, γ_cr, γ_qr, γ_cirr, es, Vr', Tr'.
+      iFrame "∗#".
       iAaccIntro with ""; try done.
       iIntros "_". iModIntro; iIntros "HΦ"; try done.
-  Qed.
+  Admitted.
 
 
 End multicopy_lsm_upsert.
